src/Abstract.v
@@ -10,7 +10,7 @@ Fixpoint abstractRun
          {I: Type -> Type}
          {A: Type}
          (abs: S)
-         (abs_step: forall (R:Type), I R -> S -> S)
+         (abs_step: forall (R:Type), I R -> R -> S -> S)
          (int: Interp I)
          (p: Program I A)
   : (A * (Interp I) * S) :=
@@ -18,7 +18,7 @@ Fixpoint abstractRun
   | ret a => (a, int, abs)
   | instr i => (evalInstruction int i,
                 execInstruction int i,
-                abs_step _ i abs)
+                abs_step _ i (evalInstruction int i) abs)
   | bind p' f => abstractRun (snd (abstractRun abs abs_step int p'))
                              abs_step
                              (snd (fst (abstractRun abs abs_step int p')))
@@ -34,7 +34,7 @@ Definition abstractExec
            {I: Type -> Type}
            {A: Type}
            (abs: S)
-           (abs_step: forall (R:Type), I R -> S -> S)
+           (abs_step: forall (R:Type), I R -> R -> S -> S)
            (int: Interp I)
            (p: Program I A)
   : Interp I :=
@@ -45,7 +45,7 @@ Definition abstractEval
            {I: Type -> Type}
            {A: Type}
            (abs: S)
-           (abs_step: forall (R:Type), I R -> S -> S)
+           (abs_step: forall (R:Type), I R -> R -> S -> S)
            (int: Interp I)
            (p: Program I A)
   : A :=
@@ -56,7 +56,7 @@ Definition deriveAbstraction
            {I: Type -> Type}
            {A: Type}
            (abs: S)
-           (abs_step: forall (R: Type), I R -> S -> S)
+           (abs_step: forall (R: Type), I R -> R -> S -> S)
            (int: Interp I)
            (p: Program I A)
   : S :=
@@ -68,7 +68,7 @@ Lemma abstract_run_run_program_same
       {A: Type}
   : forall (p: Program I A)
            (abs: S)
-           (abs_step: forall (R: Type), I R -> S -> S)
+           (abs_step: forall (R: Type), I R -> R -> S -> S)
            (int: Interp I),
     fst (abstractRun abs abs_step int p) = runProgram int p.
 Proof.
@@ -84,7 +84,7 @@ Lemma abstract_eval_eval_program_same
       {A: Type}
   : forall (p: Program I A)
            (abs: S)
-           (abs_step: forall (R: Type), I R -> S -> S)
+           (abs_step: forall (R: Type), I R -> R -> S -> S)
            (int: Interp I),
     abstractEval abs abs_step int p = evalProgram int p.
 Proof.
@@ -100,7 +100,7 @@ Lemma abstract_exec_exec_program_same
       {A: Type}
   : forall (p: Program I A)
            (abs: S)
-           (abs_step: forall (R: Type), I R -> S -> S)
+           (abs_step: forall (R: Type), I R -> R -> S -> S)
            (int: Interp I),
     abstractExec abs abs_step int p = execProgram int p.
 Proof.
