src/Contract/Temporal.v
@@ -4,7 +4,7 @@ Require Import FreeSpec.TemporalLogic.
 Require Import FreeSpec.Contract.
 
 Definition temporal_step (I: Interface) :=
-  fun (R: Type) (i: I R) => tl_step (instruction i).
+  fun (R: Type) (i: I R) (_: R) => tl_step (instruction i).
 
 Definition temporal_requirements (I: Interface) :=
   fun (R: Type) (i: I R) => instruction_satisfies (instruction i).
@@ -36,11 +36,13 @@ Definition temporal_requirements_preserves_inv
 Lemma temporal_contract_preserves_inv
       {I: Interface}
       {State: Type}
+      (promises: forall (R: Type)
+                        (i: I R),
+          R -> Formula (ISet I) -> Prop)
       (step: @PS I State)
       (inv: Formula (ISet I) -> State -> Prop)
   : temporal_requirements_preserves_inv step inv
-    -> contract_preserves_inv (temporal_requirements I)
-                              (temporal_step I)
+    -> contract_preserves_inv (temporal_contract promises)
                               inv
                               step.
 Proof.
@@ -74,9 +76,7 @@ Lemma temporal_contract_enforces_promises
                         (i: I R),
           R -> Formula (ISet I) -> Prop)
   : temporal_requirements_enforces_promises step inv promises
-    -> contract_enforces_promises (temporal_requirements I)
-                                  promises
-                                  (temporal_step I)
+    -> contract_enforces_promises (temporal_contract promises)
                                   inv
                                   step.
 Proof.
